Prove get_deref_singleton

LoadStore.v
@@ -5,20 +5,10 @@ Require Import List.
 Module Ir.
 
 
-(* get_deref_blks_byaddrs returns all alive blocks which have
-   ofss as their inbounds. *)
-Definition get_deref_blks_byaddrs (m:Ir.Memory.t) (ofss:list nat)
-: list (Ir.blockid * Ir.MemBlock.t) :=
-  List.fold_left
-           (fun blks (ofs:nat) =>
-              List.filter (fun b => Ir.MemBlock.inbounds_abs ofs b.(snd)) blks)
-           ofss
-           m.(Ir.Memory.blocks).
-
 Definition get_deref_blks_phyptr (m:Ir.Memory.t) (o:nat) (Is:list nat)
            (cid:option Ir.callid) (sz:nat)
 : list (Ir.blockid * Ir.MemBlock.t) :=
-  match (get_deref_blks_byaddrs m (o::(o+sz)::Is)) with
+  match (Ir.Memory.inbounds_blocks_all m (o::(o+sz)::Is)) with
   | nil => nil (* No such block *)
   | blks =>
     match cid with
@@ -33,23 +23,23 @@ Definition get_deref_blks_phyptr (m:Ir.Memory.t) (o:nat) (Is:list nat)
     end
   end.
 
-(* get_deref returns (block, offset) list which will be dereferenced
+(* get_deref returns (blockid, block, offset) list which will be dereferenced
    from pointer p and access size sz.
    We'll show that the list of (block, offset) is a singleton later. *)
 Definition get_deref (m:Ir.Memory.t) (p:Ir.ptrval) (sz:nat)
-: list (Ir.MemBlock.t * nat) :=
+: list (Ir.blockid * Ir.MemBlock.t * nat) :=
   match p with
   | Ir.plog (bid, ofs) => (* Logical pointer *)
     match (Ir.Memory.get m bid) with
     | None => nil (* No such block *)
     | Some blk =>
-      if Ir.MemBlock.alive blk && Ir.MemBlock.inbounds blk ofs &&
-         Ir.MemBlock.inbounds blk (ofs + sz) then
-        (blk, ofs)::nil
+      if Ir.MemBlock.alive blk && Ir.MemBlock.inbounds ofs blk &&
+         Ir.MemBlock.inbounds (ofs + sz) blk then
+        (bid, blk, ofs)::nil
       else nil
     end
   | Ir.pphy (o, Is, cid) => (* Physical pointer *)
-    List.map (fun mb => (mb, o - Ir.MemBlock.addr mb))
+    List.map (fun mb => (mb.(fst), mb.(snd), o - Ir.MemBlock.addr mb.(snd)))
              (get_deref_blks_phyptr m o Is cid sz)
   end.
 
@@ -60,31 +50,57 @@ Definition deref (m:Ir.Memory.t) (p:Ir.ptrval) (sz:nat): bool :=
 
 (* Lemma: get_deref_blks_byaddrs returns at most one alive block,
    if offsets have two disjoint numbers *)
-Lemma get_deref_blks_byaddrs_singleton:
-  forall (m:Ir.Memory.t) (m_wf:Ir.Memory.wf m) ( cid (sz:nat)
-         (bos:list Ir.MemBlock.t)
+Lemma get_deref_blks_phyptr_singleton:
+  forall (m:Ir.Memory.t) (m_wf:Ir.Memory.wf m) o Is cid sz bos
          (HSZ: 0 < sz)
          (HDEREF: get_deref_blks_phyptr m o Is cid sz = bos),
   (exists bo, bos = bo::nil) \/ (bos = nil).
 Proof.
   intros.
   unfold get_deref_blks_phyptr in HDEREF.
-  remember (Ir.Memory.inbounds_blocks m o) as blks.
-  assert (List.length blks < 3).
+  remember (Ir.Memory.inbounds_blocks_all m (o::o+sz::Is)) as blks.
+  assert (List.length blks < 2).
   {
-    apply (Ir.Memory.inbounds_blocks_atmost_2 m o).
-    assumption. congruence.
+    apply (Ir.Memory.inbounds_blocks_all_singleton2 m o (o+sz) blks Is).
+    assumption.
+    intros H.
+    destruct sz.
+    - inversion HSZ.
+    - rewrite PeanoNat.Nat.add_succ_r in H.
+      rewrite PeanoNat.Nat.add_comm in H.
+      apply PeanoNat.Nat.succ_add_discr in H.
+      assumption.
+    - congruence.
   }
   destruct blks as [| b1 blks].
   { right. simpl in HDEREF. congruence. }
-  destruct cid as [cid |].
-  - destruct (Ir.Memory.calltime m cid) as [cid' |] eqn:HCT.
-    
+  simpl in H.
+  destruct blks as [| b2 blks].
+  {
+    destruct cid as [cid |].
+    - destruct (Ir.Memory.calltime m cid) as [cid' |] eqn:HCT.
+      + simpl in HDEREF.
+        destruct (Ir.MemBlock.alive_before cid' (snd b1)).
+        * left. eexists. rewrite HDEREF. reflexivity.
+        * right. congruence.
+      + left. eexists. rewrite HDEREF. reflexivity.
+    - left. eexists. rewrite HDEREF. reflexivity.
+  }
+  {
+    simpl in H.
+    assert (S (S (length blks)) = 2 + length blks). (* -_-; *)
+    { reflexivity. }
+    rewrite H0 in H.
+    apply Lt.lt_not_le in H.
+    exfalso.
+    apply H.
+    apply PeanoNat.Nat.le_add_r.
+  }
 Qed.
 
-Lemma get_deref_singleton:
-  forall (m:Ir.Memory.t) (m_wf:Ir.Memory.wf m) (p:Ir.ptrval) (sz:nat)
-         (bos:list (Ir.MemBlock.t * nat))
+(* Theorem: get_deref always returns at most one block. *)
+Theorem get_deref_singleton:
+  forall (m:Ir.Memory.t) (m_wf:Ir.Memory.wf m) (p:Ir.ptrval) (sz:nat) bos
          (HSZ: 0 < sz)
          (HDEREF: get_deref m p sz = bos),
   (exists bo, bos = bo::nil) \/ (bos = nil).
@@ -95,14 +111,29 @@ Proof.
     destruct p as [bid ofs].
     unfold get_deref in HDEREF.
     destruct (Ir.Memory.get m bid).
-    remember (Ir.MemBlock.alive t && Ir.MemBlock.inbounds t ofs &&
-              Ir.MemBlock.inbounds t (ofs + sz)) as cond in HDEREF.
+    remember (Ir.MemBlock.alive t && Ir.MemBlock.inbounds ofs t &&
+              Ir.MemBlock.inbounds (ofs + sz) t) as cond in HDEREF.
     destruct cond; rewrite <- HDEREF.
     + left. eexists. reflexivity.
     + right. reflexivity.
     + right. congruence.
   - unfold get_deref in HDEREF.
-    
+    destruct p as (p', cid).
+    destruct p' as (o, Is).
+    remember (get_deref_blks_phyptr m o Is cid sz) as blks.
+    assert ((exists bo0, blks = bo0::nil) \/ (blks = nil)).
+    { eapply get_deref_blks_phyptr_singleton.
+      eassumption.
+      eassumption.
+      rewrite <- Heqblks. reflexivity. }
+    destruct H.
+    { destruct H.
+      rewrite H in HDEREF.
+      simpl in HDEREF.
+      left. eexists. rewrite <- HDEREF.
+      reflexivity.
+    }
+    right. rewrite H in HDEREF. simpl in HDEREF. congruence.
 Qed.
 
 
